\chapter{DISCRETE STRUCTURES}

\section{A Brief Introduction}
\textit{July 22nd.}

Discrete mathematics is primarily the study of tools for reasoning precisely the systematically about digital systems, logical problems, and combinatorial structures such as the integers, graphs, logical statements, and finite automata. Furthermore, combinatorics is the mathematics of counting and configuration; the counting, organizing, and analyzing discrete structures. 

\eax{Bloch's principle}, or Bloch's heuristics, states that every proposition on whose statement the actual infinity occurs can always be considered as a consequence of a proposition where it does not occur as a proposition on finite terms. The \eax{Ramsey principle} states that complete disorder is impossible. In any sufficiently large structure, order or regularity must emerge. These two principles may be considered complimentary to each other.

\section{Useful Methods}
The method of \eax{double counting} can be thought of a creative device or trick. Before strictly showing the statement, we utilise some examples.
\begin{example}
    Suppose we wish to show that $\sum_{k=0}^{n} \binom{n}{k} = 2^{n}$. We first ask how many ways can a subset be chosen from $\{1,2,\ldots,n\}$. The first method is to build a subset by deciding whether we want $i$ to be a part of our subset for $i \in \{1,2,...,n\}$. The second method is find the number of subsets of caridnality $i$ for $i \in \{1,2,\ldots,n\}$ and add up all the results. This leads us to conclude $2^{n} = \sum_{k=0}^{n} \binom{n}{k}$ after equating the answers from both methods.
\end{example}

\begin{theorem}[The \eax{q-binomial theorem}]
    We use the following notation:
    \begin{equation}
        \binom{n}{k}_{q} = \frac{(q^{n}-1) \cdots (q^{n-k+1}-1)}{(q^{k}-1) \cdots (q-1)}.
    \end{equation}
    Simply stated, the $q$-binomial theorem is
    \begin{equation}
        \sum_{k=0}^{n} q^{\binom{k}{2}} \binom{n}{k}_{q} z^{k} = \prod_{i=0}^{n-1} (1+q^{i}z).
    \end{equation}
\end{theorem}
The proof of the above theorem is performed by double counting; counting the number of pairs $(U,B)$ where $U$ is a $k$-dimensional subspace of $\F^{n}_{q}$ and $B$ is the flag of nested subspaces of $U$.

\subsubsection{Reccurrence Relations and Generating Functions}
Perhaps, the most important example of a recurrence relation is the Fibonacci sequence, where the terms in the sequence are defined as $F_{0} = 0$, $F_{1} = 1$, $F_{n+2} = F_{n+1} + F_{n}$ for all $n \geq 0$. Let us find the \eax{generating function} of this sequence; we start by creating
\begin{equation}
    F(t) = F_{0} + F_{1}t + F_{2}t^{2} + F_{3}t^{3} + \cdots,
\end{equation}
the generating function of $(F_{n})_{n=0}^{\infty}$. We can then work as follows---
\begin{align}
    tF(t) &= F_{0}t + F_{1}t^{2} + \cdots,\notag\\
    t^{2}F(t) &= F_{0}t^{2} + \cdots,\notag\\
    \implies (1-t-t^{2})F(t) &= t \implies F(t) = \frac{-t}{t^{2}+t-1}.
\end{align}

If we look at $F_{n+1} = 1 \cdot F_{n} + 1 \cdot F_{n-1}$ and $F_{n} = 1 \cdot F_{n} + 0 \cdot F_{n-1}$, we may notice a matrix as $\begin{bmatrix}
    F_{n+1} \\ F_{n}
\end{bmatrix} = \begin{bmatrix}
    1 & 1 \\ 1 & 0
\end{bmatrix} \begin{bmatrix}
    F_{n} \\ F_{n-1}
\end{bmatrix}$. Back substituting multiple times leads us to conclude $\begin{bmatrix}
    F_{n+1} \\ F_{n}
\end{bmatrix} = \begin{bmatrix}
    1 & 1 \\ 1 & 0
\end{bmatrix}^{n} \begin{bmatrix}
    1 \\ 0
\end{bmatrix}$. We can then diagonalize the centre matrix to decompose it as $P \begin{bmatrix}
    (1+\sqrt{5})^{n}/2^{n} & 0 \\ 0 & (1-\sqrt{5})^{n}/2^{n}
\end{bmatrix} P^{-1}$; thus, the terms of the sequence are really linear combinations of the diagonal elements that appear.

\subsubsection{Principle of Inclusion-Exclusion}
\textit{July 24th.}

Simply stated, for sets $A$ and $B$, $\# (A \cup B) = \# A + \# B + \# (A \cap B)$. For three sets $A, B$ and $C$, we have
$\# (A \cup B \cup C) = \# A + \# B + \# C - \# (A \cap B) - \# (B \cap C) - \# (A \cap C) + \# (A \cap B \cap C)$. This can be extended to any finite number of finite sets.

\begin{theorem}[The \eax{principle of inclusion-exclusion}]
    Let $S$ be an $N$-set ($\#S = N$), and let $E_{1},E_{2},\ldots,E_{r}$ be, not necessarily distinct, subsets of $S$. For any subset $M$ of the indexing set $\{1,2,\ldots,r\}$, let $N(M)$ denote the number of elements of $S$ in $\bigcap_{i \in M} E_{i}$, and for $0 \leq j \leq r$, define
    \begin{align}
        N_{j} = \sum_{\# M = j} N(M).
    \end{align}
    Then the number of elements of $S$ not in any of the $E_{i}$'s is
    \begin{align}
        \#(S \setminus \bigcup_{i = 1}^{r} E_{i}) = N - N_{1} + N_{2} - N_{3} + \cdots + (-1)^{r} N_{r}.
    \end{align}
\end{theorem}
\begin{proof}
    For $x \in S$, define $M:S \to \{0,1\}$ as $M(x) = 1$ if $x \in \bigcap_{i \in M} E_{i}$ and $0$ otherwise. Thus,
    \begin{align}
        \sum_{x \in S} M(x) = \# (\bigcap_{i \in M} E_{i}) = N(M) \implies N_{j} = \sum_{\# M = j} \sum_{x \in S} M(x) = \sum_{x \in S} \sum_{\# M = j} M(x).
    \end{align}
    The alternating sum then becomes
    \begin{align}
        \sum_{x \in S} 1 - \sum_{x \in S} \sum_{\# M = 1} M(x) + \cdots + (-1)^{r} \sum_{x \in S} \sum_{\# M = r} M(x) = \sum_{x \in S} \left( 1 - \sum_{\# M = 1} M(x) + \cdots + (-1)^{r} \sum_{\# M = r} M(x) \right).
    \end{align}
    Call the term within the parentheses as $F(x)$. We deal with cases; if $x \notin \bigcup_{i=1}^{r} E_{i}$, then $F(x) = 1$. If $x$ is in exactly $k \geq 1$ of the sets $E_{1},E_{2},\ldots,E_{r}$, then
    \begin{align}
        F(x) = 1 - \binom{k}{1} + \binom{k}{2} - \binom{k}{3} + \cdots + (-1)^{k} \binom{k}{k} = (1-1)^{k} = 0.
    \end{align}
    This is independent of $k$; we conclude that the alternating sum reduces to the number of elements in $S$ not in any of the $E_{i}$'s.
\end{proof}

\begin{corollary}
    Retaining notation from the previous theorem, if $S = \bigcup_{i=1}^{r} E_{r}$, then
    \begin{align}
        N = N_{1} - N_{2} + \cdots + (-1)^{r-1} N_{r}.
    \end{align}
\end{corollary}

We look at some examples of the principle in use.
\begin{example}
    Let $d_{n}$ be the number of permutations $\pi$ of the set $\{1,2,\ldots,n\}$ such that $\pi(i) \neq i$ for all $1 \leq i \leq n$. Such a permutation is called a \eax{derangement}, where no point is fixed. We wish to count all such permutations. Let the set of all permutations of the set be $S$. Let $E_{i}$ denote the set of all permutations that fix $i$, for $1 \leq i \leq n$. Thus, $S$ without $\bigcup_{i=1}^{n} E_{i}$ would then denote the set of all derangements. Making use of the principle, we have
    \begin{align}
        \#(S \setminus \bigcup_{i=1}^{n} E_{i}) = n! - \binom{n}{1}(n-1)! + \binom{n}{2} (n-2)! - \cdots = n! \left( 1-\frac{1}{1!} + \frac{1}{2!} - \frac{1}{3!} + \cdots + (-1)^{n} \frac{1}{n!} \right)
    \end{align}
    which is approximately $\frac{n!}{e}$ for larger $n$. Thus, the probability of choosing a derangemnet is $e^{-1}$.
\end{example}

\begin{example}
    Suppose we have two sets $X$ and $Y$ with $\# X = n$ and $\# Y = k$. We ask how many surjective maps exists from $X$ to $Y$. The set $S$, this time, is the set of all functions from $X$ to $Y$, being $Y^{X}$. $E_{i}$ denotes the set of functions from $X$ to $Y$ such that $y_{i}$ is not in the image of $X$. The elments within $S$ not in any of the $E_{i}$'s are surjective maps. Clearly, $N_{i} = \binom{k}{i} (k-i)^{n}$, and the cardinality of $S \setminus \bigcup_{i=1}^{k} E_{i}$ is then
    \begin{align}
        \sum_{i=0}^{k} (-1)^{i} \binom{k}{i} (k-i)^{n}.
    \end{align}
\end{example}

\begin{example}
    We wish to show that the expression $\sum_{i=0}^{n} (-1)^{i} \binom{n}{i} \binom{m+n-i}{k-i}$ evaluates to $\binom{m}{k}$ if $m \geq k$, and $0$ otherwise. To this end, fix $X = \{x_{1},\ldots,x_{n}\}$ and $Y = \{y_{1},\ldots,y_{m}\}$ and set $Z = X \cup Y$. We now ask how many $k$-subsets of $Z$ consist of only points form $Y$. Let $S$ be the set of all $k$-subsets of $Z$, and denote $E_{i}$ to be the set of $k$-subsets of $Z$ containing $x_{i}$ for $1 \leq i \leq n$. The left hand side of our inclusion-exclusion principle evaluates to $\binom{m+n}{k}$. Each $N_{i}$ evaluates to $\binom{n}{i} \binom{m+n-i}{k-i}$, proving our expression above.
\end{example}

The next example relates to the Euler totient function.

\begin{example}
    Recall that, from the \eax{fundamental theorem of arithmetic}, each natural number may be expressed uniquely (upto order) as the product of distinct primes raised to values, that is, $n = p_{1}^{a_{1}} \cdots p_{r}^{a_{r}}$. The \eax{Euler totient function} $\phi: \N \to \C$ acts on the naturals and returns $\phi(n)$, the number of positive integers $k \leq n$ such that $\gcd (k,n) = 1$. Certainly, $\phi(p) = p-1$ for a prime $p$. Our task is to find a closed form formula for $\phi(n)$.

    Set $S = \{1,2,\ldots,n\}$, and set $E_{i}$ to be the set of integers in $S$ divisible by $p_{i}$ for $1 \leq i \leq r$. Clearly, the value $\# (S \setminus \bigcup_{i=1}^{r} E_{i})$ returns the set of all numbers in $\{1,2,\ldots,n\}$ coprime to $n$. Note that $N = n$. The value of $N_{1}$ is $\sum_{i=1}^{r} \frac{n}{p_{i}}$ , the value of $N_{2}$ is is $\sum_{1 \leq i \leq j \leq r} \frac{n}{p_{i}p_{j}}$. The cloesd form formula then becomes
    \begin{align}
        \phi(n) = \# (S \setminus \bigcup_{i=1}^{r} E_{i}) = n - n \sum_{i=1}^{r} \frac{1}{p_{i}} + n \sum_{1 \leq i \leq j \leq r} \frac{1}{p_{i}p_{j}} + \cdots = n\left( 1-\frac{1}{p_{1}} \right)\left( 1-\frac{1}{p_{2}} \right) \cdots \left( 1-\frac{1}{p_{r}} \right).
    \end{align}
\end{example}


\subsubsection{Number Theory}
We continue with the Euler totient function.
\begin{theorem}
    $\sum \limits_{d \mid n} \phi(d) = n$.
\end{theorem}
\begin{proof}
    For each integer $m \in \{1, 2, \ldots, n\}$, the value $\gcd(m, n)$ is a divides $n$. Fix a divisor $d$ of $n$. The number of integers $m$ such that $\gcd(m, n) = d$ is equal to the number of integers $m$ such that $\gcd\left(\frac{m}{d}, \frac{n}{d}\right) = 1$, where $\frac{m}{d}$ runs over integers between $1$ and $\frac{n}{d}$.
    Therefore, the number of such $m$ is $\phi\left(\frac{n}{d}\right)$. Summing over all divisors $d$ of $n$, we get:
    \[
        n = \sum_{d \mid n} \phi\left(\frac{n}{d}\right)
    \]
    which is the same as $\sum_{d \mid n} \phi(d)$.
\end{proof}

The \eax{M\"obius function} is defined as
\begin{equation}
    \mu(d) \defeq \begin{cases}
        1, &\text{ if } d \text{ is a product of even number of distinct primes},\\
        -1, &\text{ if } d \text{ is a product of odd number of distinct primes},\\
        0, &\text{ if otherwise; the number } d \text{ is square-free.}
    \end{cases}
\end{equation}

\begin{theorem}
    \begin{align}
        \sum_{d \mid n} \mu(d) = \begin{cases}
            1, &\text{ if } n = 1,\\
            0, &\text{ if otherwise.}
        \end{cases}
    \end{align}
\end{theorem}

\begin{proof}
    For $n = 1$, it is clear. For $n > 1$, rewriting $n$ as $p_{1}^{a_{1}} \cdots p_{r}^{a_{r}}$ helps us see that
    \begin{align}
        \sum_{d \mid n} \mu(d) = 1 - \binom{r}{1} + \binom{r}{2} - \binom{r}{3} + \cdots = (1-1)^{r} = 0.
    \end{align}
\end{proof}

This property of the M\"obius function proves to be useful.

\begin{theorem}[The \eax{M\"obius inversion formula}]
    Suppose we have two function $f: \N \to \R$ and $g:\N \to \R$ which relate as
    \begin{align}
        f(n) = \sum_{d \mid n} g(d).
    \end{align}
    Then the function $g$ satisfies
    \begin{align}
        g(n) = \sum_{d \mid n} \mu\left( \frac{n}{d} \right)f(d).
    \end{align}
\end{theorem}
The proof of this is left as an exercise to the reader.

\begin{example}
    Let $N_{n}$ denote the number of circular sequences of $n$ $0$'s and $1$'s, modulo rotation. Let us explicitly find out $N_{n}$.
\end{example}